James C - free vars

isabelle/Chapter09.thy
@@ -17,9 +17,42 @@ where "free_vars (Var v) = {v}"
     | "free_vars Zero = {}"
     | "free_vars (Succ e) = free_vars e"
     | "free_vars (Rec e0 e1 et) = free_vars e0 Un free_vars et Un 
-          ((%x. case x of 0 => 0 | Suc 0 => 0 | Suc (Suc k) => k) ` free_vars e1)"
-    | "free_vars (Lam t b) = (%x. case x of 0 => 0 | Suc k => k) ` free_vars b"
+          ((%x. case x of 0 => undefined | Suc 0 => undefined | Suc (Suc k) => k) ` (free_vars e1 - {0, 1}))"
+    | "free_vars (Lam t b) = (%x. case x of 0 => undefined | Suc k => k) ` (free_vars b - {0})"
     | "free_vars (Ap e1 e2) = free_vars e1 Un free_vars e2"
+
+lemma lam_frees: "(n : free_vars (Lam r b)) = (Suc n : free_vars b)" 
+proof auto
+  fix x
+  assume "x : free_vars b"
+     and "Suc (case x of 0 => undefined | Suc k => k) ~: free_vars b"
+  thus "x = 0" by (cases x, simp_all)
+next
+  assume "Suc n : free_vars b"
+  moreover have "n = nat_case undefined (%k. k) (Suc n)" by simp
+  ultimately show "n \<in> nat_case undefined (\<lambda>k. k) ` (free_vars b - {0})" by blast
+qed
+
+lemma rec_frees: "(n : free_vars (Rec e0 e1 e)) = (n : free_vars e0 | n : free_vars e | Suc (Suc n) : free_vars e1)"
+proof auto
+  fix x
+  assume B: "Suc (Suc (case x of Suc (Suc k) => k)) ~: free_vars e1"
+     and C: "x : free_vars e1"
+     and "0 < x"
+  thus "x = Suc 0"
+  proof (cases x, simp)
+  case (Suc x')
+    with C B show ?thesis by (cases x', simp_all)
+  qed
+next
+  assume "Suc (Suc n) : free_vars e1"
+     and "n ~: free_vars e0"
+     and "n ~: nat_case undefined (nat_case undefined (%k. k)) ` (free_vars e1 - {0, Suc 0})"
+  moreover have "n = nat_case undefined (nat_case undefined (%k. k)) (Suc (Suc n)) ==> 
+          (Suc (Suc n)):(free_vars e1 - {0, Suc 0}) ==> 
+              n : nat_case undefined (nat_case undefined (%k. k))`(free_vars e1 - {0, Suc 0})" by blast
+  ultimately show "n : free_vars e" by simp
+qed
 
 primrec incr_from :: "nat => expr => expr"
 where "incr_from n (Var v) = Var (if v < n then v else Suc v)"
@@ -29,6 +62,14 @@ where "incr_from n (Var v) = Var (if v < n then v else Suc v)"
     | "incr_from n (Lam t b) = Lam t (incr_from (Suc n) b)"
     | "incr_from n (Ap e1 e2) = Ap (incr_from n e1) (incr_from n e2)"
 
+primrec sub_from :: "nat => expr => expr"
+where "sub_from n (Var v) = Var (if v < n then v else if v = n then undefined else v - 1)"
+    | "sub_from n Zero = Zero"
+    | "sub_from n (Succ e) = Succ (sub_from n e)"
+    | "sub_from n (Rec e0 e1 et) = Rec (sub_from n e0) (sub_from (Suc (Suc n)) e1) (sub_from n et)"
+    | "sub_from n (Lam t b) = Lam t (sub_from (Suc n) b)"
+    | "sub_from n (Ap e1 e2) = Ap (sub_from n e1) (sub_from n e2)"
+
 primrec subst :: "expr => expr => nat => expr"
 where "subst (Var v) e x = (if v = x then e else Var v)"
     | "subst Zero e x = Zero"
@@ -36,6 +77,22 @@ where "subst (Var v) e x = (if v = x then e else Var v)"
     | "subst (Rec e0 e1 et) e x = Rec (subst e0 e x) (subst e1 (incr_from 0 (incr_from 0 e)) (Suc (Suc x))) (subst et e x)"
     | "subst (Lam t b) e x = Lam t (subst b (incr_from 0 e) (Suc x))"
     | "subst (Ap e1 e2) e x = Ap (subst e1 e x) (subst e2 e x)"
+
+lemma [simp]: "free_vars (subst e e' x) = (if x : free_vars e then free_vars e - {x} Un free_vars e' else free_vars e)"
+proof (induction e arbitrary: e' x)
+case Var
+  thus ?case by simp
+next case Zero
+  thus ?case by simp
+next case Succ
+  thus ?case by simp
+next case (Rec e0 e1 e)
+  thus ?case sorry
+next case (Lam t b)
+  thus ?case sorry
+next case (Ap e1 e2)
+  thus ?case sorry
+qed
 
 inductive typecheck :: "(nat, type) assoc => expr => type => bool"
 where tvar [simp]: "lookup env v = Some t ==> typecheck env (Var v) t"
@@ -88,37 +145,27 @@ next case (tapp env e1 t2 t e2)
   ultimately show ?case by simp
 qed
 
-lemma typecheck_nofree: "typecheck env e t ==> k ~: free_vars e ==> typecheck (extend env k v) e t"
-proof (induction env e t arbitrary: k rule: typecheck.induct)
-case tvar
-  thus ?case by simp
+lemma [simp]: "typecheck (extend_at env n k) e t ==> n ~: free_vars e ==> typecheck env (sub_from n e) t"
+proof (induction "extend_at env n k" e t arbitrary: env n rule: typecheck.induct)
+case (tvar v t)
+  thus ?case by (cases "v < n", simp, cases "v = n", simp_all)
 next case tzer
   thus ?case by simp
 next case tsuc
   thus ?case by simp
-next case (trec env e e0 t e1)
-  have "Suc (Suc k) ~: free_vars e1"
-  proof auto
-    assume "Suc (Suc k) : free_vars e1"
-    hence "!!f. k = f (Suc (Suc k)) ==> k : f`free_vars e1" by simp
-    with trec show False by simp
-  qed
-  with trec show ?case by simp
-next case (tlam env r b t)
-  hence "Suc k ~: free_vars b"
-  proof auto
-    assume "Suc k : free_vars b"
-    hence "!!f. k = f (Suc k) ==> k : f`free_vars b" by simp
-    with tlam show False by simp
-  qed
-  with tlam show ?case by simp
-next case (tapp env e1 t2 t e2)
-  from tapp have "typecheck (extend env k v) e1 (Arr t2 t)" by simp
-  moreover from tapp have "typecheck (extend env k v) e2 t2" by simp
+next case (trec e e0 t e1)
+  from trec have "n ~: free_vars (Rec e0 e1 e)" by simp
+  hence "Suc (Suc n) ~: free_vars e1" apply (auto simp add: rec_frees) sorry
+  with trec show ?case by (simp add: extend_at_swap)
+next case (tlam r b t)
+  thus ?case apply (simp add: extend_at_swap lam_frees) sorry
+next case (tapp e1 t2 t e2)
+  from tapp have "typecheck env (sub_from n e1) (Arr t2 t)" by simp
+  moreover from tapp have "typecheck env (sub_from n e2) t2" by simp
   ultimately show ?case by simp
-qed 
+qed
 
-lemma typecheck_subst: "typecheck (extend env x t') e t ==> typecheck env e' t' ==> typecheck env (subst e e' x) t"
+lemma [simp]: "typecheck (extend env x t') e t ==> typecheck env e' t' ==> typecheck env (subst e e' x) t"
 proof (induction "extend env x t'" e t arbitrary: env e' x rule: typecheck.induct)
 case tvar
   thus ?case by auto
@@ -148,7 +195,7 @@ inductive eval :: "expr => expr => bool"
 where esuc [simp]: "eval n n' ==> eval (Succ n) (Succ n')"
     | eap1 [simp]: "eval e1 e1' ==> eval (Ap e1 e2) (Ap e1' e2)"
     | eap2 [simp]: "is_val e1 ==> eval e2 e2' ==> eval (Ap e1 e2) (Ap e1 e2')"
-    | eap3 [simp]: "is_val e2 ==> eval (Ap (Lam t b) e2) (subst b e2 0)"
+    | eap3 [simp]: "is_val e2 ==> eval (Ap (Lam t b) e2) (sub_from 0 (subst b e2 0))"
     | erc1 [simp]: "eval e e' ==> eval (Rec e0 e1 e) (Rec e0 e1 e')"
     | erc2 [simp]: "eval (Rec e0 e1 Zero) e0"
     | erc3 [simp]: "is_val e ==> eval (Rec e0 e1 (Succ e)) (subst (subst e1 e 1) (Rec e0 e1 e) 0)"
@@ -160,27 +207,35 @@ lemma canonical_arr: "typecheck env e (Arr t1 t2) ==> is_val e ==> (EX v. e = La
 by (induction e, auto)
 
 theorem preservation: "eval e e' ==> typecheck env e t ==> typecheck env e' t"
-proof (induction e e' arbitrary: t rule: eval.induct)
+proof (induction e e' arbitrary: t env rule: eval.induct)
 case (esuc n n')
   moreover from esuc have "t = Nat" by (simp add: inv_suc)
   moreover from esuc have "typecheck env n Nat" by (simp add: inv_suc)
   ultimately show ?case by simp
 next case (eap1 e1 e1' e2)
-  with eap1 have "EX t2. typecheck env e1' (Arr t2 t) & typecheck env e2 t2" by (auto simp add: inv_app)
+  hence "EX t2. typecheck env e1' (Arr t2 t) & typecheck env e2 t2" by (auto simp add: inv_app)
   thus ?case by auto
 next case eap2
   thus ?case by auto
 next case (eap3 e2 r b)
-  hence "typecheck env (Ap (Lam r b) e2) t" by simp
+  hence "typecheck (extend_at env 0 r) b t & typecheck env e2 r" by (auto simp add: inv_app inv_lam)
+  hence "typecheck (extend_at env 0 r) b t" by simp
 
-  have "typecheck env (subst b e2 0) t" sorry
-  thus ?case by simp
+  moreover have "typecheck (extend_at env 0 k) e2 r" sorry
+  ultimately have "typecheck (extend_at env 0 k) (subst b e2 0) t" by simp
+
+
+  moreover have  "0 ~: (if 0 : free_vars b then free_vars b - {0} Un free_vars e2 else free_vars b)" sorry 
+  ultimately show ?case by simp
 next case erc1
   thus ?case by auto
 next case (erc2 e0 e1)
   from erc2 have "typecheck env Zero Nat & typecheck env e0 t & typecheck (extend_at (extend_at env 0 Nat) 0 t) e1 t" by (rule inv_rec)
   thus ?case by simp
 next case (erc3 e e0 e1)
+
+
+
   thus ?case sorry
 qed
 
@@ -197,14 +252,23 @@ next case (tsuc env n)
     thus ?thesis by simp
   next case False
     from tsuc False have "\<exists>a. eval n a" by simp
+
+
+
     hence "\<exists>a. eval (Succ n) (Succ a)" sorry
     thus ?thesis by auto
   qed
 next case trec
+
+
+
   thus ?case sorry
 next case tlam
   thus ?case by simp
 next case tapp
+
+
+
   thus ?case sorry
 qed 
 
